påbörjat labb 2

CircularBuffer.dfy
@@ -7,11 +7,86 @@ class CircularMemory{
 
 
     constructor Init(cap : int)
-    //missing some pre-conditions here
+        requires cap > 0
+        ensures Valid()
     {
         cells := new int[cap];
         read_position, write_position := 0, 0;
         isFlipped := false;
     }
 
+    predicate Valid() 
+        reads this
+    {
+        (read_position >= 0 && read_position < cells.Length) &&
+        (write_position >= 0 && write_position < cells.Length) &&
+        (cells.Length > 0)
+        //(read_position % cells.Length < cells.Length) && (read_position % cells.Length >= 0)
+        //(isFlipped ==> write_position < read_position) &&
+        //(!isFlipped ==> write_position >= read_position) 
+    }
+
+    // A predicate indicating no more Read available
+    predicate isEmpty()
+        reads this
+        requires Valid()
+        ensures Valid()
+    {
+        (read_position == write_position)
+    }
+
+    //A predicate indicating no more Write should be allowed
+    predicate isFull()
+        reads this
+        requires Valid()
+        ensures Valid()
+    {
+        (write_position + 1 % cells.Length == read_position)
+    }
+
+    method Read() returns (isSuccess : bool, content : int)
+        modifies this
+        requires Valid()
+        ensures  Valid()
+        ensures isSuccess  ==> read_position == old(read_position) + 1 % cells.Length 
+        ensures isSuccess  ==> content       == cells[old(read_position)]
+        ensures !isSuccess ==> read_position == old(read_position)
+        ensures !isSuccess ==> content       == -100
+    {
+        isSuccess := false;
+        content := -100;
+
+        if(!(write_position + 1 % cells.Length == read_position)){
+            if(read_position >= 0 && read_position < cells.Length){
+                content       := cells[read_position];
+                read_position := read_position + 1 % cells.Length;
+                isSuccess     := true;
+                return isSuccess, content;  
+            }
+        }else { 
+            return isSuccess, -100;
+        }
+    }
 }
+    /*
+    method Write(input : int) returns (isSuccess : bool)
+        modifies this
+        requires Valid()
+        requires isFull()
+        ensures  Valid()
+        ensures isFull()
+        ensures  isSuccess ==> cells[write_position] == input
+        ensures !isSuccess ==> cells[write_position] != input
+    
+    {
+        if(!isFull()){
+            return false;
+        } else if(write_position == read_position){
+            cells[write_position] := input;
+            write_position := write_position + 1;
+            return true;
+        } else {
+            return false;
+        }
+    }
+    */
